\documentclass[a4paper,12pt]{article}

\usepackage{amsmath}

\begin{document}

\section*{MATH 3225 - HW1 Solutions}

\begin{enumerate}
	
	\item $(A \cup B)^c = (\{2, 4, 6\} \cup \{4, 5, 6\})^c = \{2, 4, 5, 6\}^c = \{1, 3\} \\
	A^c \cap B^c = \{2, 4, 6\}^c \cap \{4, 5, 6\}^c = \{1, 3, 5\} \cap \{1, 2, 3\} = \{1, 3\} \\
	(A \cap B)^c = (\{2, 4, 6\} \cap \{4, 5, 6\})^c = \{4, 6\}^c = \{1, 2, 3, 5\} \\
	A^c \cup B^c = \{2, 4, 6\}^c \cup \{4, 5, 6\}^c = \{1, 3, 5\} \cup \{1, 2, 3\} = \{1, 2, 3, 5\}$
	
	\setcounter{enumi}{7}
	\item Let $P_i$ denote the probability of winning against opponent $i$, and let $a_1, a_2, a_3$ denote the ordering of opponents in a particular tournament. Due to the Inclusion-Exclusion Principle, the probability of winning the second game in addition to at least one of the remaining games is
		\[ P_{a_2} (P_{a_1} + P_{a_3} - P_{a_1} P_{a_3}) = P_{a_1} P_{a_2} + P_{a_2} P_{a_3} - P_{a_1} P_{a_2} P_{a_3}. \]
	Because $P_2 > P_1$ and $P_2 > P_3$, the expression is maximized when $a_2 = 2$. In addition, the expression is equivalent for $(a_1, a_3) = (1, 3)$ and $(a_3, a_1) = (3, 1)$.
	
	\item (a) Using the distributive law and (the finite-element version of) the third axiom of probability measure,
	\begin{align*}
		A &= A \cap \Omega \\
		&= A \cap \bigcup_{i = 1}^{n} S_i \\
		&= \bigcup_{i = 1}^{n} (A \cap S_i) \\
		&= \sum_{i = 1}^{n} P(A \cap S_i).
	\end{align*}
	(b) One example partition of $\Omega$ is $\{B, B^c \cap C, B^c \cap C^c\}$, and using part (a),
		\[ P(A) = P(A \cap B) + P(A \cap B^c \cap C) + P(A \cap B^c \cap C^c). \]
	Combining the fact that
		\[ (A \cap B^c \cap C) \cup (A \cap B \cap C) = (B^c \cup B) \cap (A \cap C) = A \cap C \]
	with another application of the third axiom to get
		\[ P(A \cap B^c \cap C) + P(A \cap B \cap C) = P(A \cap C), \]
	we have
		\[ P(A) = P(A \cap B) + P(A \cap C) + P(A \cap B^c \cap C^c) - P(A \cap B \cap C). \]

	\item Applying the third axiom and the fact from part (9b),
	\begin{align*}
		P((A \cap B^c) \cup (A^c \cap B)) &= P(A \cap B^c) + P(A^c \cap B) \\
		&= \left( P(A) - P(A \cap B) \right) + \left( P(B) - P(B \cap A) \right) \\
		&= P(A) + P(B) - 2P(A \cap B)
	\end{align*}

	\setcounter{enumi}{15}
	\item Let $A$ be the event in which the coin with two different faces was chosen, and let $B$ be the event in which the result was heads. Then
	\begin{align*}
		P(A | B) &= \frac{P(A) P(B | A)}{P(B)} \\
		&= \frac{(1 / 3) (1 / 2)}{(1 / 3) (1 + 0 + 1 / 2)} \\
		&= \frac{1}{3}
	\end{align*}
	
	\item
	\[ \left( \frac{95}{100} \right) \left( \frac{94}{99} \right) \left( \frac{93}{98} \right) \left( \frac{92}{97} \right) = \frac{636709}{784245} \]
	
	\setcounter{enumi}{18}
	\item Let $A$ be the event in which the paper is in drawer $j$, and let $B$ be the event in which Alice unsuccessfully searches drawer $i$ (which means that either drawer $i$ does not contain the paper, or drawer $i$ contains the paper but Alice does not find it). Then
	\begin{align*}
		P(A | B) &= \frac{P(A) P(B | A)}{P(B)} \\
		&= \frac{p_j P(B | A)}{(1 - p_i) + p_i(1 - d_i)} \\
		&= \frac{p_j P(B | A)}{1 - p_id_i}
	\end{align*}
	In the case that the term paper is in drawer $j$ for $j \neq i$ in event $A$, a search in drawer $i$ will always be unsuccessful, so $P(B | A) = 1$. For $i = j$, the term paper must be in drawer $i$ and the chance that the search is unsuccessful is $P(B | A) = 1 - d_i$.

\end{enumerate}

\end{document}