\documentclass[a4paper,12pt]{article}

\usepackage{amsfonts, amsmath, amssymb, amsthm, enumitem, fancyhdr, graphicx}
\usepackage[margin=1in, includehead, includefoot, heightrounded]{geometry}
\allowdisplaybreaks
\pagestyle{fancy}
\rhead{Erick Lin}

\newcommand{\norm}[1]{\left\lVert#1\right\rVert}
\renewcommand{\thesubsection}{\arabic{subsection}}
\newtheorem{theorem}{Theorem}
\newtheorem{lemma}[theorem]{Lemma}

\begin{document}

\section*{MATH 4640 -- HW2 Solutions}
\begin{enumerate}
    \item
        Let $p_k(x)$ be the polynomial interpolation at $f(x_0), \cdots, f(x_k)$, and let $q(x) = f(x) - p_k(x)$, noting that $q(x) = 0$ for all $x = x_0, \cdots, x_k$. Taking the $k$th derivative on each side gives $q^{(k)}(x) = f^{(k)}(x) - p_k^{(k)}(x)$. Since $q$ has $k + 1$ roots in the interval $(a, b)$, $q^{(k)}$ must have at least one root $\xi \in (a, b)$ by Rolle's theorem, meaning that $f^{(k)}(\xi) - p_k^{(k)}(\xi) = 0$. \par
        Note that $f[x_0, \cdots, x_k]$ is the leading coefficient of $p_k$ and $p_k$ has degree $k$, which means that $p_k^{(k)}(x) = f[x_0, \cdots, x_k]k!$ everywhere. The result then follows from substituting this into the previous relation.

    \item
        \begin{align*}
            g_1(x) = \begin{cases}
                1.4 + \frac{0.6 - 1.4}{1 - 0}x, &0 \leq x \leq 1 \\
                0.6 + \frac{1.0 - 0.6}{2 - 1}(x - 1), &1 \leq x \leq 2 \\
                1.0 + \frac{0.6 - 1.0}{3 - 2}(x - 2), &2 \leq x \leq 3 \\
                0.6 + \frac{1.0 - 0.6}{4 - 3}(x - 3), &3 \leq x \leq 4
            \end{cases}
            = \begin{cases}
                1.4 - 0.8x, &0 \leq x \leq 1 \\
                0.2 + 0.4x, &1 \leq x \leq 2 \\
                1.8 - 0.4x, &2 \leq x \leq 3 \\
                -0.6 + 0.4x, &3 \leq x \leq 4
            \end{cases}
        \end{align*}

    \item
        We want to solve
        \begin{align*}
            \left[ \begin{array}{ccccc}
                    2 & \lambda_0 & 0 & 0 & 0 \\
                    \mu_1 & 2 & \lambda_1 & 0 & 0 \\
                    0 & \mu_2 & 2 & \lambda_2 & 0 \\
                    0 & 0 & \mu_3 & 2 & \lambda_3 \\
                    0 & 0 & 0 & \mu_4 & 2
            \end{array} \right]
            \left[ \begin{array}{c}
                    M_0 \\
                    M_1 \\
                    M_2 \\
                    M_3 \\
                    M_4
            \end{array} \right]
            =
            \left[ \begin{array}{c}
                    d_0 \\
                    d_1 \\
                    d_2 \\
                    d_3 \\
                    d_4
            \end{array} \right]
        \end{align*}
        for the $M_i$, where $\mu_i = \frac{x_i - x_{i - 1}}{x_{i + 1} - x_{i - 1}}$, $\lambda_i = 1 - \mu_i = \frac{x_{i + 1} - x_i}{x_{i + 1} - x_{i - 1}}$, and
        \begin{align*}
            d_i = \begin{cases}
                6f[x_0, x_0, x_1], &i = 0 \\
                6f[x_{i - 1}, x_i, x_{i + 1}], &1 \leq i \leq n - 1 \\
                6f[x_{n - 1}, x_n, x_n], &i = n.
            \end{cases}
        \end{align*}
        It is easy to see that $\mu_1 = \mu_2 = \mu_3 = 0.5$, $\mu_4 = 1$, $\lambda_0 = 1$, and $\lambda_1 = \lambda_2 = \lambda_3 = 0.5$. We also have, noting $f[x_0, x_0] = f'(0)$ and $f[x_4, x_4] = f'(4)$, that
        \begin{align*}
            f[x_0, x_0, x_1] &= \frac{f[x_0, x_1] - f[x_0, x_0]}{x_1 - x_0} = \frac{\frac{0.6 - 1.4}{1 - 0} - 1}{1 - 0} = -1.8 \\
            f[x_0, x_1, x_2] &= \frac{f[x_1, x_2] - f[x_0, x_1]}{x_2 - x_0} = \frac{\frac{1.0 - 0.6}{2 - 1} - \frac{0.6 - 1.4}{1 - 0}}{2 - 0} = 0.6 \\
            f[x_1, x_2, x_3] &= \frac{f[x_2, x_3] - f[x_1, x_2]}{x_3 - x_1} = \frac{\frac{0.6 - 1.0}{3 - 2} - \frac{1.0 - 0.6}{2 - 1}}{3 - 1} = -0.4 \\
            f[x_2, x_3, x_4] &= \frac{f[x_3, x_4] - f[x_2, x_3]}{x_4 - x_2} = \frac{\frac{1.0 - 0.6}{4 - 3} - \frac{0.6 - 1.0}{3 - 2}}{4 - 2} = 0.4 \\
            f[x_3, x_4, x_4] &= \frac{f[x_4, x_4] - f[x_3, x_4]}{x_4 - x_3} = \frac{-1 - \frac{1.0 - 0.6}{4 - 3}}{4 - 3} = -1.4,
        \end{align*}
        so the system of equations becomes
        \begin{align*}
            \left[ \begin{array}{ccccc}
                    2 & 1 & 0 & 0 & 0 \\
                    0.5 & 2 & 0.5 & 0 & 0 \\
                    0 & 0.5 & 2 & 0.5 & 0 \\
                    0 & 0 & 0.5 & 2 & 0.5 \\
                    0 & 0 & 0 & 1 & 2
            \end{array} \right]
            \left[ \begin{array}{c}
                    M_0 \\
                    M_1 \\
                    M_2 \\
                    M_3 \\
                    M_4
            \end{array} \right]
            =
            \left[ \begin{array}{c}
                    -10.8 \\
                    3.6 \\
                    -2.4 \\
                    2.4 \\
                   -8.4 
            \end{array} \right],
        \end{align*}
        and thus we have $M_0 = -7.657, M_1 = 4.514, M_2 = -3.2, M_3 = 3.486$, and $M_4 = -5.943$ approximately. \par
        Using the formula
        \begin{align*}
            S(x)|_{[x_{i - 1}, x_i]} &= M_{i - 1} \frac{(x_i - x)^3}{6(x_i - x_{i - 1})} + M_i \frac{(x - x_{i - 1})^3}{6(x_i - x_{i - 1})} \\
            &+ \left( y_{i - 1} - \frac{M_{i - 1} \left( x_i - x_{i - 1} \right)^2}{6} \right) \frac{x_i - x}{x_i - x_{i - 1}} + \left( y_i - \frac{M_i (x_i - x_{i - 1})^2}{6} \right) \frac{x - x_{i - 1}}{x_i - x_{i - 1}}
        \end{align*}
        gives, approximately,
        \begin{align*}
            S(x) = \begin{cases}
                2.029x^3 - 3.829x^2 + x + 1.4, &0 \leq x \leq 1 \\
                -1.226x^3 - 5.754x^2 - 8.282x + 4.354, &1 \leq x \leq 2 \\
                1.114x^3 - 8.286x^2 + 19.858 - 14.486, &2 \leq x \leq 3 \\
                -1.572x^3 + 15.887x^2 - 52.66x + 58.032, &3 \leq x \leq 4.
            \end{cases}
        \end{align*}

    \item
        Since $|f(x) - p_3(x)| = \frac{f^{(4)}(\xi)}{4!}(x - x_0)(x - x_1)(x - x_2)(x - x_3)$ for any $\xi \in (x_0, x_3)$, we have that $|f'(x) - p_3'(x)| = \frac{f^{(4)}(\xi)}{4!} \sum_{i = 0}^3 \prod_{j \neq i}^3 (x - x_j)$. In other words,
        \begin{align*}
            |f'(x) - p_3'(x)| &\leq \frac{1}{24} \max_{x_0 \leq \xi \leq x_3} f^{(4)}(\xi) \max_{x_0 \leq x \leq x_3} \sum_{i = 0}^3 \prod_{j \neq i}^3 (x - x_j) \\
            &\leq \frac{1}{24} \max_{x_0 \leq \xi \leq x_3} f^{(4)}(\xi) \sum_{i = 0}^3 \left( \frac{x_3 - x_0}{2} \right)^2 \\
            &= \frac{1}{24} \max_{x_0 \leq \xi \leq x_3} f^{(4)}(\xi) \left( \frac{4 \cdot 27h^3}{8} \right) \\
            &= \frac{9h^3}{16} \max_{x_0 \leq \xi \leq x_3} f^{(4)}(\xi).
        \end{align*}

    \item
        Write $p(x) = m_0 + m_1 x + m_2 x^2$ so that the objective is to solve for $m_0$, $m_1$, and $m_2$. The constraints respectively give us the relations
        \begin{gather}
            m_0 + m_1 x_0 + m_2 x_0^2 = a \\
            m_1 + 2m_2 x_0 = b \\
            m_1 + 2m_2 x_1 = c.
        \end{gather}
        Relations (2) and (3) give $m_2 = \frac{c - b}{2(x_1 - x_0)}$ and $m_1 = c - \frac{x_1(c - b)}{x_1 - x_0}$. Lastly, substitution into (1) gives $m_0 = a - cx_0 - \frac{(c - b)x_0^2}{x_1 - x_0} + \frac{x_0 x_1 (c - b)}{x_1 - x_0}$.

    \item
        Given $y = 8$, $z = 2$, the interpolating polynomial is $f(x) = -\frac{4x^4}{3} + \frac{25x^3}{6} + \frac{4x^2}{3} - \frac{31x}{6} + 1$.
    \item
    \item
        The well-definedness and continuity of $p(x)$, $p'(x)$, and $p''(x)$ at $x = 0$ respectively require that $a = 0$, $b = 0$, and $c = 0$. Any $d \neq 0$ is sufficient for $p(x)$ to be a cubic spline because it is then of degree $3$ and satisfies the continuity of the second derivative everywhere.
\end{enumerate}

\end{document}
