\documentclass[a4paper,12pt]{article}

\usepackage{amsfonts, amsmath, amssymb, amsthm, enumitem, fancyhdr, mathtools, physics}
\usepackage[margin=3.5cm]{geometry}
\allowdisplaybreaks
\pagestyle{fancy}
\rhead{Erick Lin}

\renewcommand{\thesubsection}{\arabic{subsection}}
%\DeclarePairedDelimiterX{\norm}[1]{\lVert}{\rVert}{#1}
\newcommand{\bs}{\boldsymbol}
\newtheorem{theorem}{Theorem}
\newtheorem{lemma}[theorem]{Lemma}
\theoremstyle{remark}
\newtheorem{remark}{Remark}

\begin{document}

\section*{MATH 4441 -- HW5 Solutions}
\begin{enumerate}
    \item[1.]
        The first and second partial derivatives are given by
        \begin{gather*}
            \bs{f}_u = (\cos v, \sin v, 1) \quad
            \bs{f}_v = (-u\sin v, u\cos v, 0) \\
            \bs{f}_{uu} = (0, 0, 0) \quad
            \bs{f}_{uv} = \bs{f}_{vu} = (-\sin v, \cos v, 0) \quad 
            \bs{f}_{vv} = (-u\cos v, -u\sin v, 0)
        \end{gather*}
        and the normal vector to the surface at $(u, v)$ is given by
        \begin{align*}
            \bs{N}(u, v) &= \frac{\bs{f}_u \times \bs{f}_v}{\norm{\bs{f}_u \times \bs{f}_v}} = \frac{(-u\cos v, -u\sin v, u\cos^2v + u\sin^2v)}{\sqrt{2}u} \\
            &= \frac{(-\cos v, -\sin v, 1)}{\sqrt{2}},
        \end{align*}
        so we have that
        \begin{gather*}
            \bs{f}_{uu} = 0\bs{f}_u + 0\bs{f}_v + 0\bs{N}(u, v) \\
            \bs{f}_{uv} = \bs{f}_{vu} = 0\bs{f}_u + \frac{1}{u}\bs{f}_v + 0\bs{N}(u, v) \\
            \bs{f}_{vv} = -\frac{u}{2}\bs{f}_u + 0\bs{f}_v + \sqrt{2}u\bs{N}(u, v),
        \end{gather*}
        which shows that the Christoffel symbols are given by
        \begin{gather*}
            \Gamma_{11}^1 =
            \Gamma_{11}^2 = 0 \\
            \Gamma_{12}^1 = 0 \quad
            \Gamma_{12}^2 = \frac{1}{u} \\
            \Gamma_{22}^1 = -\frac{u}{2} \quad
            \Gamma_{22}^2 = 0.
        \end{gather*}

    \item[2.]
        The first fundamental form is given by
        \begin{align*}
            \left[ \begin{array}{cc}
                    g_{11} & g_{12} \\
                    g_{21} & g_{22}
            \end{array} \right]
            = \left[ \begin{array}{cc}
                    \bs{f}_u \cdot \bs{f}_u & \bs{f}_u \cdot \bs{f}_v \\
                    \bs{f}_v \cdot \bs{f}_u & \bs{f}_v \cdot \bs{f}_v
            \end{array} \right]
            = \left[ \begin{array}{cc}
                    2 & 0 \\
                    0 & u^2
            \end{array} \right]
        \end{align*}
        and thus
        \begin{align*}
            \left[ \begin{array}{cc}
                    g^{11} & g^{12} \\
                    g^{21} & g^{22}
            \end{array} \right]
            = \left[ \begin{array}{cc}
                    g_{11} & g_{12} \\
                    g_{21} & g_{22}
            \end{array} \right]^{-1}
            = \frac{1}{2u^2}
            \left[ \begin{array}{cc}
                    u^2 & 0 \\
                    0 & 2
            \end{array} \right]
            = \left[ \begin{array}{cc}
                    1/2 & 0 \\
                    0 & 1/u^2
            \end{array} \right].
        \end{align*}
        Recall that the formula for the Christoffel symbols is
        \begin{align*}
            \Gamma_{jk}^i = \sum_{l = 1}^2 g^{il} \frac{1}{2} \left( (g_{kl})_{u_j} + (g_{lj})_{u_k} - (g_{jk})_{u_l} \right)
        \end{align*}
        where $u_1 = u$ and $u_2 = v$. Substituting for each result, we have
        \begin{gather*}
            \Gamma_{11}^1 = \sum_{l = 1}^2 g^{1l} \frac{1}{2} \left( (g_{1l})_{u_1} + (g_{l1})_{u_1} - (g_{11})_{u_l} \right) = g^{11} \frac{1}{2} (g_{11})_u = 0 \\
            \Gamma_{11}^2 = \sum_{l = 1}^2 g^{2l} \frac{1}{2} \left( (g_{1l})_{u_1} + (g_{l1})_{u_1} - (g_{11})_{u_l} \right) = g^{22} \frac{1}{2} \left( -(g_{11})_v \right) = 0 \\
            \Gamma_{12}^1 = \sum_{l = 1}^2 g^{1l} \frac{1}{2} \left( (g_{2l})_{u_1} + (g_{l1})_{u_2} - (g_{12})_{u_l} \right) = g^{11} \frac{1}{2} (g_{11})_v = 0 \\
            \Gamma_{12}^2 = \sum_{l = 1}^2 g^{2l} \frac{1}{2} \left( (g_{2l})_{u_1} + (g_{l1})_{u_2} - (g_{12})_{u_l} \right) = g^{22} \frac{1}{2} (g_{22})_u = \frac{1}{u} \\
            \Gamma_{22}^1 = \sum_{l = 1}^2 g^{1l} \frac{1}{2} \left( (g_{2l})_{u_2} + (g_{l2})_{u_2} - (g_{22})_{u_l} \right) = g^{11} \frac{1}{2} \left( -(g_{22})_u \right) = -\frac{u}{2} \\
            \Gamma_{22}^2 = \sum_{l = 1}^2 g^{2l} \frac{1}{2} \left( (g_{2l})_{u_2} + (g_{l2})_{u_2} - (g_{22})_{u_l} \right) = g^{22} \frac{1}{2} \left( -(g_{22})_v \right) = 0.
        \end{gather*}
        From above, we also obtain the formulas for when $g$ is any diagonal matrix.

    \item[3.]
        \begin{enumerate}
            \item
                Since
                \begin{gather*}
                    \left[ \begin{array}{cc}
                            g^{11} & g^{12} \\
                            g^{21} & g^{22}
                    \end{array} \right]
                    = \frac{(1 + u^2 + v^2)^2}{4}
                    \left[ \begin{array}{cc}
                            1 & 0 \\
                            0 & 1
                    \end{array} \right], \\
                    \left[ \begin{array}{cc}
                            g_{11} & g_{12} \\
                            g_{21} & g_{22}
                    \end{array} \right]_u
                    = -\frac{16u}{(1 + u^2 + v^2)^3}
                    \left[ \begin{array}{cc}
                            1 & 0 \\
                            0 & 1
                    \end{array} \right], \\
                    \left[ \begin{array}{cc}
                            g_{11} & g_{12} \\
                            g_{21} & g_{22}
                    \end{array} \right]_v
                    = -\frac{16v}{(1 + u^2 + v^2)^3}
                    \left[ \begin{array}{cc}
                            1 & 0 \\
                            0 & 1
                    \end{array} \right],
                \end{gather*}
                we have that
                \begin{gather*}
                    \Gamma_{11}^1 = -\frac{2u}{1 + u^2 + v^2} \quad
                    \Gamma_{11}^2 = \frac{2v}{1 + u^2 + v^2} \\
                    \Gamma_{12}^1 = -\frac{2v}{1 + u^2 + v^2} \quad
                    \Gamma_{12}^2 = -\frac{2u}{1 + u^2 + v^2} = \Gamma_{21}^2 \\
                    \Gamma_{22}^1 = \frac{2u}{1 + u^2 + v^2} \quad
                    \Gamma_{22}^2 = -\frac{2v}{1 + u^2 + v^2},
                \end{gather*}
                and thus the Gauss curvature is
                \begin{align*}
                    K &= \frac{1}{g_{11}} \left[ (\Gamma_{11}^2)_v - (\Gamma_{12}^2)_u + \Gamma_{11}^1 \Gamma_{12}^2 + \Gamma_{11}^2 \Gamma_{22}^2 - \Gamma_{12}^1 \Gamma_{21}^2 - (\Gamma_{12}^2)^2 \right] \\
                    &= \frac{(1 + u^2 + v^2)^2}{4} \biggl[ -\frac{4v^2}{(1 + u^2 + v^2)^2} - \frac{4u^2}{(1 + u^2 + v^2)^2} + \frac{4u^2}{(1 + u^2 + v^2)^2} \\
                    &\qquad- \frac{4v^2}{(1 + u^2 + v^2)^2} - \frac{4uv}{(1 + u^2 + v^2)^2} - \frac{4u^2}{(1 + u^2 + v^2)^2} \biggr] \\
                    &= -(u^2 + uv + 2v^2).
                \end{align*}

            \item
                Since
                \begin{gather*}
                    \left[ \begin{array}{cc}
                            g^{11} & g^{12} \\
                            g^{21} & g^{22}
                    \end{array} \right]
                    = \frac{(1 - (u^2 + v^2))^2}{4}
                    \left[ \begin{array}{cc}
                            1 & 0 \\
                            0 & 1
                    \end{array} \right], \\
                    \left[ \begin{array}{cc}
                            g_{11} & g_{12} \\
                            g_{21} & g_{22}
                    \end{array} \right]_u
                    = \frac{16u}{(1 - (u^2 + v^2))^3}
                    \left[ \begin{array}{cc}
                            1 & 0 \\
                            0 & 1
                    \end{array} \right], \\
                    \left[ \begin{array}{cc}
                            g_{11} & g_{12} \\
                            g_{21} & g_{22}
                    \end{array} \right]_v
                    = \frac{16v}{(1 - (u^2 + v^2))^3}
                    \left[ \begin{array}{cc}
                            1 & 0 \\
                            0 & 1
                    \end{array} \right],
                \end{gather*}
                we have that
                \begin{gather*}
                    \Gamma_{11}^1 = \frac{2u}{1 - (u^2 + v^2)} \quad
                    \Gamma_{11}^2 = \frac{2v}{1 - (u^2 + v^2)} \\
                    \Gamma_{12}^1 = \frac{2v}{1 - (u^2 + v^2)} \quad
                    \Gamma_{12}^2 = \frac{2u}{1 - (u^2 + v^2)} = \Gamma_{21}^2 \\
                    \Gamma_{22}^1 = \frac{2u}{1 - (u^2 + v^2)} \quad
                    \Gamma_{22}^2 = \frac{2v}{1 - (u^2 + v^2)},
                \end{gather*}
                and thus the Gauss curvature is
                \begin{align*}
                    K &= \frac{1}{g_{11}} \left[ (\Gamma_{11}^2)_v - (\Gamma_{12}^2)_u + \Gamma_{11}^1 \Gamma_{12}^2 + \Gamma_{11}^2 \Gamma_{22}^2 - \Gamma_{12}^1 \Gamma_{21}^2 - (\Gamma_{12}^2)^2 \right] \\
                    &= \frac{(1 - (u^2 + v^2))^2}{4} \biggl[ \frac{4v^2}{(1 - (u^2 + v^2))^2} + \frac{4u^2}{(1 - (u^2 + v^2))^2} + \frac{4u^2}{(1 - (u^2 + v^2))^2} \\
                    &\qquad+ \frac{4v^2}{(1 - (u^2 + v^2))^2} + \frac{4uv}{(1 - (u^2 + v^2))^2} + \frac{4u^2}{(1 - (u^2 + v^2))^2} \biggr] \\
                    &= 3u^2 + uv + 2v^2.
                \end{align*}

            \item
                Since
                \begin{gather*}
                    \left[ \begin{array}{cc}
                            g^{11} & g^{12} \\
                            g^{21} & g^{22}
                    \end{array} \right]
                    = v^2
                    \left[ \begin{array}{cc}
                            1 & 0 \\
                            0 & 1
                    \end{array} \right], \\
                    \left[ \begin{array}{cc}
                            g_{11} & g_{12} \\
                            g_{21} & g_{22}
                    \end{array} \right]_u
                    = \left[ \begin{array}{cc}
                            0 & 0 \\
                            0 & 0
                    \end{array} \right], \\
                    \left[ \begin{array}{cc}
                            g_{11} & g_{12} \\
                            g_{21} & g_{22}
                    \end{array} \right]_v
                    = -\frac{2}{v^3}
                    \left[ \begin{array}{cc}
                            1 & 0 \\
                            0 & 1
                    \end{array} \right],
                \end{gather*}
                we have that
                \begin{gather*}
                    \Gamma_{11}^1 = 0 \quad
                    \Gamma_{11}^2 = \frac{1}{v} \\
                    \Gamma_{12}^1 = -\frac{1}{v} \quad
                    \Gamma_{12}^2 = 0 = \Gamma_{21}^2 \\
                    \Gamma_{22}^1 = \frac{1}{v} \quad
                    \Gamma_{22}^2 = -\frac{1}{v},
                \end{gather*}
                and thus the Gauss curvature is
                \begin{align*}
                    K &= \frac{1}{g_{11}} \left[ (\Gamma_{11}^2)_v - (\Gamma_{12}^2)_u + \Gamma_{11}^1 \Gamma_{12}^2 + \Gamma_{11}^2 \Gamma_{22}^2 - \Gamma_{12}^1 \Gamma_{21}^2 - (\Gamma_{12}^2)^2 \right] \\
                    &= v^2 \left[ -\frac{1}{v^2} - 0 + 0 - \frac{1}{v^2} - 0 - 0^2 \right] \\
                    &= -2.
                \end{align*}
        \end{enumerate}

    \item[4.]
        \begin{enumerate}
            \item
                \begin{align*}
                    \text{Area}(D_\rho) &= \int_{-\rho}^\rho \int_{-\sqrt{\rho^2 - v^2}}^{\sqrt{\rho^2 - v^2}} \sqrt{\det g} \dd{u} \dd{v} \\
                    &= \int_{-\rho}^\rho \int_{-\sqrt{\rho^2 - v^2}}^{\sqrt{\rho^2 - v^2}} \frac{4}{(1 - (u^2 + v^2))^2} \dd{u} \dd{v}
                \end{align*}
            \item
                The boundary curve is parameterized by $(u(t), v(t)) = \rho(\cos t, \sin t)$, and thus its length is given by
                \begin{align*}
                    \text{Length}(\partial D_\rho) &= \int_0^{2\pi} \sqrt{ g_{11} \left( \dv{u}{t} \right)^2 + 2g_{12} \dv{u}{t} \dv{v}{t} + g_{22} \left( \dv{v}{t} \right)^2 } \dd{t} \\
                    &= \int_0^{2\pi} \sqrt{ \frac{4}{(1 - (u^2 + v^2))^2}\sin^2 t + \frac{4}{(1 - (u^2 + v^2))^2}\cos^2 t } \dd{t} \\
                    &= \int_0^{2\pi} \frac{2}{1 - \rho^2} \dd{t} = \frac{4\pi}{1 - \rho^2}.
                \end{align*}
            \item
                First,
                \begin{align*}
                    \text{Area}(D_\rho) &= \int_{-\rho}^\rho \int_{-\sqrt{\rho^2 - v^2}}^{\sqrt{\rho^2 - v^2}} \sqrt{\det g} \dd{u} \dd{v} \\
                    &= \int_{-\rho}^\rho \int_{-\sqrt{\rho^2 - v^2}}^{\sqrt{\rho^2 - v^2}} \frac{4}{(1 + u^2 + v^2)^2} \dd{u} \dd{v}.
                \end{align*}
                Using the same parametrization of the boundary as before,
                \begin{align*}
                    \text{Length}(\partial D_\rho) &= \int_0^{2\pi} \sqrt{ g_{11} \left( \dv{u}{t} \right)^2 + 2g_{12} \dv{u}{t} \dv{v}{t} + g_{22} \left( \dv{v}{t} \right)^2 } \dd{t} \\
                    &= \int_0^{2\pi} \sqrt{ \frac{4}{(1 + u^2 + v^2)^2}\sin^2 t + \frac{4}{(1 + u^2 + v^2)^2}\cos^2 t } \dd{t} \\
                    &= \int_0^{2\pi} \frac{2}{1 + \rho^2} \dd{t} = \frac{4\pi}{1 + \rho^2}.
                \end{align*}
        \end{enumerate}

    \item[5.]
        The result follows directly from applying the Theorema Egregium. Alternatively, since
        \begin{gather*}
            \left[ \begin{array}{cc}
                    g^{11} & g^{12} \\
                    g^{21} & g^{22}
            \end{array} \right]
            = \left[ \begin{array}{cc}
                    1/\lambda & 0 \\
                    0 & 1/\lambda
            \end{array} \right], \\
            \left[ \begin{array}{cc}
                    g_{11} & g_{12} \\
                    g_{21} & g_{22}
            \end{array} \right]_u
            = \left[ \begin{array}{cc}
                    \partial\lambda/\partial u & 0 \\
                    0 & \partial\lambda/\partial u
            \end{array} \right], \\
            \left[ \begin{array}{cc}
                    g_{11} & g_{12} \\
                    g_{21} & g_{22}
            \end{array} \right]_v
            = \left[ \begin{array}{cc}
                    \partial\lambda/\partial v & 0 \\
                    0 & \partial\lambda/\partial v
            \end{array} \right],
        \end{gather*}
        we have that
        \begin{gather*}
            \Gamma_{11}^1 = \frac{1}{2\lambda} \pdv{\lambda}{u} \quad
            \Gamma_{11}^2 = -\frac{1}{2\lambda} \pdv{\lambda}{v} \\
            \Gamma_{12}^1 = \frac{1}{2\lambda} \pdv{\lambda}{v} \quad
            \Gamma_{12}^2 = \frac{1}{2\lambda} \pdv{\lambda}{u} = \Gamma_{21}^2 \\
            \Gamma_{22}^1 = -\frac{1}{2\lambda} \pdv{\lambda}{u} \quad
            \Gamma_{22}^2 = \frac{1}{2\lambda} \pdv{\lambda}{v},
        \end{gather*}
        and thus the Gauss curvature is
        \begin{align*}
            K &= \frac{1}{g_{11}} \left[ (\Gamma_{11}^2)_v - (\Gamma_{12}^2)_u + \Gamma_{11}^1 \Gamma_{12}^2 + \Gamma_{11}^2 \Gamma_{22}^2 - \Gamma_{12}^1 \Gamma_{21}^2 - (\Gamma_{12}^2)^2 \right] \\
            &= \frac{1}{\lambda} \biggl[ \left( -\frac{1}{2\lambda} \pdv[2]{\lambda}{v} + \frac{1}{2\lambda^2} \left( \pdv{\lambda}{v} \right)^2 \right) - \left( \frac{1}{2\lambda} \pdv[2]{\lambda}{u} - \frac{1}{2\lambda^2} \left( \pdv{\lambda}{u} \right)^2 \right) \\
            &\qquad\qquad+ \left( \frac{1}{2\lambda} \pdv{\lambda}{u} \right)^2 - \left( \frac{1}{2\lambda} \pdv{\lambda}{v} \right)^2 - \frac{1}{(2\lambda)^2} \pdv{\lambda}{u} \pdv{\lambda}{v} - \left( \frac{1}{2\lambda} \pdv{\lambda}{u} \right)^2 \biggr] \\
            &= -\frac{1}{2\lambda} \left[ \frac{\partial^2}{\partial v^2}\ln\lambda + \frac{\partial^2}{\partial u^2}\ln\lambda \right] = -\frac{1}{2\lambda} \nabla^2(\ln\lambda).
        \end{align*}

    \item[6.]
        For the unit sphere, the Gauss curvature is $1/1^2 = 1$, and the first fundamental form is $\left[ \begin{array}{cc}
                \sin^2 v & 0 \\
                0 & 1
        \end{array} \right]$, which has determinant $\sin^2 v$. Then the total curvature is given by
        \begin{align*}
            \int_{S^2} K(p) \dd{A} = \int_{-\pi}^\pi \int_0^{2\pi} \sin v \dd{u} \dd{v} = 4\pi.
        \end{align*}
\end{enumerate}

\end{document}
